casestudy/coding_wolfSSL_proof_BL_CL.ec
@@ -5,29 +5,35 @@ require Coding_wolfSSL.
 import StdOrder.IntOrder Ring.IntID.
 
 clone import Coding_wolfSSL.T with
-theory LeakageModel <-  LeakageModelTV.
+theory LeakageModel <-  LeakageModelCL.
 
 (* input base64decode is public and (base64decode % 64 == 0) 
    input c is secret *)
-(* need to take the pre condition as sub-lemmas *)
+  (* need to take the pre condition as sub-lemmas *)
 equiv l_final : M.base64_Char2Val_jazz ~ M.base64_Char2Val_jazz :
 ={M.leakages} /\ (base64Decode{1} = base64Decode{2}) /\
 (0 <= to_uint (c{1} - (of_int 43)%W8) < 80) /\
-(0 <= to_uint (c{2} - (of_int 43)%W8) < 80) /\
-(of_int (to_uint ((c{1} - (of_int 43)%W8) `&` (of_int 63)%W8)))%W64 =
-(of_int (to_uint ((c{2} - (of_int 43)%W8) `&` (of_int 63)%W8)))%W64 /\
-(of_int (to_uint ((c{1} - (of_int 43)%W8) `&` (of_int 15)%W8 `|` (of_int 64)%W8)))%W64 =
-(of_int (to_uint ((c{2} - (of_int 43)%W8) `&` (of_int 15)%W8 `|` (of_int 64)%W8)))%W64
-  ==> ={M.leakages}.
+(0 <= to_uint (c{2} - (of_int 43)%W8) < 80)
+==> ={M.leakages}.
 proof.
 proc; inline *; auto; rewrite /=.
-move=> &1 &2 [] hleak [] hp [] h1 [] h2 [] h3 h4 /=. split=> //=.
+move=> &1 &2 [] hleak [] hp [] h1 h2 /=. split=> //=.
 + rewrite hp. case: h1=> h1 h1'. case: h2=> h2 h2'.
-  by rewrite /leak_mem /= /leak_mem_id /= /zeroextu64 /= h4.
-rewrite hp /=. rewrite /leak_mem /= /leak_mem_id /=.
-split=> //=. rewrite /zeroextu64 /=. by rewrite h3 /=.
-qed.
-
-  
-  
-
+  rewrite /leak_mem /= /leak_mem_CL /=. rewrite !offset_div.
+  + admit.
+  + admit.
+  + admit.
+  + admit.
+  + admit.
+  + admit.
+  by auto.
+rewrite hp /=. rewrite /leak_mem /= /leak_mem_CL /=.
+split=> //=. rewrite !offset_div.
++ admit.
++ admit.
++ admit.
++ admit.
++ admit.
++ admit.
+by auto.
+admitted.
